\documentclass[12pt]{article}
\usepackage{amsmath}
\usepackage{amsfonts}

% :vim set makeprg=pdflatex notes:

\begin{document}

\newcommand{\dt}[0]{\partial_t}
\newcommand{\phase}[0]{e^{-i\int_0^tE_n(t')dt'}}
\newcommand{\wps}[0]{|\psi(t)\rangle}
\newcommand{\wpsn}[0]{|\psi_n(t)\rangle}
\newcommand{\awpsm}[0]{\langle\psi_n(t)|}
\newcommand{\wPs}[0]{|\Psi(t)\rangle}

\section{Four types of fourier transform}
\begin{eqnarray}{1\over2\pi}\int_{-\infty}^\infty dxe^{ikx} &=& \delta(k) \\
{1\over2\pi}\int_0^{2\pi}dxe^{ikx} &=& \delta_{k0}\mbox{, }k\mbox{ integer} \\
{1\over N}\sum_{m=0}^{N-1}e^{2\pi ikm/N} &=& \sum_{i=-\infty}^\infty\delta_{k,iN}\mbox{, }k\mbox{ integer} \\
{1\over L}\sum_{k=-\infty}^\infty e^{2\pi ikx/L} &=& \sum_{i=-\infty}^\infty\delta(x-kL) \\
\end{eqnarray}

% From PHYSICAL R E~VI EW VOLUME 168, NUM HER 3 15 AP R IL 1968 Dynamics of Electrons in Solids in External Fields J. ZAK*
\section{Fourier transform of operators}
\begin{eqnarray}&& \int d\alpha d\beta\exp(i\alpha\hat{p}+i\beta\hat{x})\operatorname{tr}(f(\hat{x},\hat{p})\exp(-i\alpha\hat{p}-i\beta\hat{x}))|x\rangle \\
&=& \int d\alpha d\beta\operatorname{tr}(f(\hat{x},\hat{p})\exp(-i\alpha\hat{p}-i\beta\hat{x}))\exp(i\alpha\hat{p}+i\beta\hat{x})|x\rangle \\
&=& \int d\alpha d\beta\operatorname{tr}(f(\hat{x},\hat{p})\exp(-i\alpha\hat{p})exp(-i\beta\hat{x}))\exp(i\beta\hat{x})\exp(i\alpha\hat{p})|x\rangle \\
&=& \int d\alpha d\beta\operatorname{tr}(f(\hat{x},\hat{p})\exp(-i\alpha\hat{p})exp(-i\beta\hat{x}))\exp(i\beta\hat{x})|x+\alpha\rangle \\
&=& \int d\alpha d\beta\operatorname{tr}(f(\hat{x},\hat{p})\exp(-i\alpha\hat{p})exp(-i\beta\hat{x}))\exp(i\beta(x+\alpha))|x+\alpha\rangle \\
&=& \int d\alpha d\beta dx'\langle x'|f(\hat{x},\hat{p})\exp(-i\alpha\hat{p})exp(-i\beta\hat{x})|x'\rangle\exp(i\beta(x+\alpha))|x+\alpha\rangle \\
&=& \int d\alpha d\beta dx'\langle x'|f(\hat{x},\hat{p})\exp(-i\alpha\hat{p})exp(-i\beta x')|x'\rangle\exp(i\beta(x+\alpha))|x+\alpha\rangle \\
&=& \int d\alpha d\beta dx'\langle x'|f(\hat{x},\hat{p})\exp(-i\beta x')|x'-\alpha\rangle\exp(i\beta(x+\alpha))|x+\alpha\rangle \\
&=& \int d\alpha d\beta dx'\langle x'|f(\hat{x},\hat{p})|x'-\alpha\rangle\exp(i\beta(x-x'+\alpha))|x+\alpha\rangle \\
&=& \int d\alpha dx'\langle x'|f(\hat{x},\hat{p})|x'-\alpha\rangle\delta(x-x'+\alpha)|x+\alpha\rangle \\
&=& \int dx'\langle x'|f(\hat{x},\hat{p})|x'-x'+x\rangle\delta(x-x'+\alpha)|x+x'-x\rangle \\
&=& \int dx'\langle x'|f(\hat{x},\hat{p})|x\rangle|x'\rangle \\
&=& \int dx'|x'\rangle\langle x'|f(\hat{x},\hat{p})|x\rangle \\
&=& f(\hat{x},\hat{p})|x\rangle \\
\end{eqnarray}

\section{Fermi-Dirac Statistics}
\begin{eqnarray}g_i &=& \mbox{number of possible states at level } i\\
n_i &=& \mbox{number of particles at level } i\\
n_i\mbox{ particles into }g_i\mbox{ states} &=& {g_i! \over n_i!(g_i-n_i)!}\\
Z &=& \prod_i{g_i! \over n_i!(g_i-n_i)!}\\
\log Z &=& \mbox{const}-\sum_i(\log{n!}-\log(g_i-n_i)!)\\
&\approx& \mbox{const}-\sum_i(n_i\log n_i-n_i+(g_i-n_i)\log(g_i-n_i)-g_i+n_i)\\
\end{eqnarray}

\begin{eqnarray}
W &=& \mbox{const}-\sum_i(n_i\log n_i-n_i+(g_i-n_i)\log(g_i-n_i)-g_i+n_i)+\alpha(N-\sum_in_i)+\beta(E-\sum_i\epsilon_in_i) \\
{\partial W\over\partial n_i} &=& -(\log n_i+1-1-\log(g_i-n_i)-1+1)-\alpha-\beta\epsilon_i \\
\log(g_i-n_i)-\log n_i &=& \alpha+\beta\epsilon_i \\
\log(g_i/n_i-1) &=& \alpha+\beta\epsilon_i \\
g_i/n_i-1 &=& \exp{(\alpha+\beta\epsilon_i)} \\
n_i &=& {g_i\over1+\exp{(\alpha+\beta\epsilon_i)}} \\
\end{eqnarray}

\section{The Adiabatic Theorem}
Schr\"odinger equation:
\begin{equation}
\label{eq:schrod}
i\hbar\dt\wpsn=H(t)\wpsn
\end{equation}

Consider $\phase\wpsn$. Not a solution as

\[
i\dt\phase\wpsn \ne H(t)\phase\wpsn
\]

LHS:
\begin{eqnarray*}
& & (i\cdot(-i)E_n(t)\phase+i\phase\dt)\wpsn \\
& = & \phase(E_n(t)+i\dt)\wpsn
\end{eqnarray*}

RHS:
\[
E_n(t)\phase\wpsn
\]

Mismatch of: $\phase i\dt\wpsn$.

Expand wavefunction $\wPs$ in terms of $\phase\wpsn$ anyway:
\[
\wPs = \sum_nc_n(t)\phase\wpsn
\]

Substitute in \ref{eq:schrod}:

LHS:
\[
\sum_nc_n(t)\phase E_n(t)\wpsn
\]
RHS:
\begin{eqnarray*}
& & i\hbar\sum_n((\dt c_n(t))\phase\wpsn + c_n(t)(-iE_n(t))\phase\wpsn+ \\
& &                                      + c_n(t)\phase\dt\wpsn \\
&=& (i\hbar\dt c_n(t)+c_n(t)E_n(t))\phase\wpsn+c_n(t)\phase\dt\wpsn
\end{eqnarray*}

\[
\sum_nc_n(t)\phase i\hbar\wpsn+i\hbar(\dt c_n(t))\phase\wpsn = 0
\]

\subsection{Differentiating the energy}
\[
H(t)\wpsn=E_n(t)\wpsn
\]

Differentiating this:
\[
(\dt H(t))\wpsn+H_n(t)\dt\wpsn=(\dt E_n(t))\wpsn+E_n(t)\dt\wpsn
\]
LHS:

\begin{eqnarray*}
& & \awpsm(\dt H(t))\wpsn+\awpsm H_n(t)\dt\wpsn \\
&=& \awpsm(\dt H(t))\wpsn+E_m(t)\awpsm\dt\wpsn
\end{eqnarray*}
RHS:

\[
\dt E_n(t)+E_n(t)\awpsm\dt\wpsn
\]

Therefore:
\[
\awpsm(\dt H(t))\wpsn+(E_m(t)-E_n(t))\awpsm\dt\wpsn=\delta_{mn}\dt E_n(t)
\]

If $m\ne n$:

\[
\awpsm\dt\wpsn={\awpsm(\dt -H(t))\wpsn \over E_n(t)-E_m(t)}
\]

% http://www.phy.cuhk.edu.hk/course/2011-2012/2/phys5410/download/0/Lecture10%20Adiabatic%20evolution%20and%20Berry%20phase.pdf
% page 9 still needed

\section{Kubo Formula}
\begin{eqnarray}i{\partial\over\partial t}|\psi\rangle &=& H|\psi\rangle\\
i{\partial\over\partial t}|\psi'\rangle &=& H'|\psi'\rangle\\
|\psi'\rangle &=&|\psi\rangle+|\delta\psi\rangle\\
H' &=&H+\delta H(t)\\
i{\partial\over\partial t}(|\psi\rangle+|\delta\psi\rangle) &=& (H+\delta H(t))|(\psi\rangle+|\delta\psi\rangle)\\
i{\partial\over\partial t}(|\psi\rangle+|\delta\psi\rangle) &=& H|(\psi\rangle+|\delta\psi\rangle)+\delta H(t)|(\psi\rangle+|\delta\psi\rangle)\\
i{\partial\over\partial t}|\delta\psi\rangle &=& H|\delta\psi\rangle+\delta H(t)|\psi\rangle+O(\delta^2)\\
i({\partial\over\partial t}+iH)|\delta\psi\rangle &=& \delta H(t)|\psi\rangle\\
\exp(iHt)i({\partial\over\partial t}+iH)|\delta\psi\rangle &=& \exp(iHt)\delta H(t)|\psi\rangle\\
i{\partial\over\partial t}\exp(iHt)|\delta\psi\rangle &=& \exp(iHt)\delta H(t)|\psi\rangle\\
i\exp(iHt)|\delta\psi\rangle &=& \int dt'\exp(iHt')\delta H(t')|\psi\rangle\\
|\delta\psi\rangle &=& -i\int dt'\exp(iH(t'-t))\delta H(t')|\psi\rangle\\
\langle\psi'|B|\psi'\rangle &=& (\langle\psi|+\langle\delta\psi|)B(|\psi\rangle+|\delta\psi\rangle)\\
\delta \langle\psi'|B|\psi'\rangle &=& \langle\psi|B|\delta\psi\rangle+\langle\delta\psi|B|\psi\rangle\\
\delta\langle\psi'|B|\psi'\rangle &=& -i\int dt'\langle\psi(t)|B\exp(iH(t'-t))\delta H(t')|\psi(t')\rangle+\langle\delta\psi|B|\psi\rangle\\
\delta\langle\psi'|B|\psi'\rangle &=& -i\int dt'\langle\psi(t)|B\exp(iH(t'-t))\delta H(t')\exp(-iH(t'-t))\exp(iH(t'-t))|\psi(t')\rangle+\langle\delta\psi|B|\psi\rangle\\
\delta\langle\psi'|B|\psi'\rangle &=& -i\langle\psi(t)|\int dt'B\exp(iH(t'-t))\delta H(t')\exp(-iH(t'-t))|\psi(t)\rangle+\langle\delta\psi|B|\psi\rangle\\
\delta\langle\psi'|B|\psi'\rangle &=& -i\langle\psi(t)|\int dt'[B,\exp(iH(t'-t))\delta H(t')\exp(-iH(t'-t))]|\psi(t)\rangle\\
\delta\langle\psi'|B|\psi'\rangle &=& -i\langle\int dt'[B,\exp(iH(t'-t))\delta H(t')\exp(-iH(t'-t))]\rangle\\
\end{eqnarray}

-------------------------

\begin{eqnarray}i{\partial\over\partial t}|\psi\rangle &=& H|\psi\rangle\\
i\exp(iHt)|\delta\psi\rangle &=& \int dt'\exp(iHt')\delta H(t')|\psi\rangle\\
|\delta\psi\rangle &=& -i\int dt'\exp(iH(t'-t))\delta H(t')|\psi\rangle\\
\langle\psi'|B|\psi'\rangle &=& (\langle\psi|+\langle\delta\psi|)B(|\psi\rangle+|\delta\psi\rangle)\\
\delta \langle\psi'|B|\psi'\rangle &=& \langle\psi|B|\delta\psi\rangle+\langle\delta\psi|B|\psi\rangle\\
\delta\langle\psi'|B|\psi'\rangle &=& -i\int dt'\langle\psi(t)|B\exp(iH(t'-t))\delta H(t')|\psi(t')\rangle+\langle\delta\psi|B|\psi\rangle\\
\delta\langle\psi'|B|\psi'\rangle &=& -i\int dt'\langle\psi(t)|\exp(iH(t'-t))\exp(-iH(t'-t))B\exp(iH(t'-t))\delta H(t')|\psi(t')\rangle+\langle\delta\psi|B|\psi\rangle\\
\delta\langle\psi'|B|\psi'\rangle &=& -i\int dt'\langle\psi(t')|\exp(-iH(t'-t))B\exp(iH(t'-t))\delta H(t')|\psi(t')\rangle+\langle\delta\psi|B|\psi\rangle\\
\hat{B}(t,t') &=& \exp(-iH(t'-t))B\exp(iH(t'-t))\\
\delta\langle\psi'|B|\psi'\rangle &=& -i\int dt'\langle\psi(t')|\hat{B}(t,t')\delta H(t')|\psi(t')\rangle+\langle\delta\psi|B|\psi\rangle\\
\delta\langle\psi'|B|\psi'\rangle &=& -i\langle\int dt'[\hat{B}(t,t'),\delta H(t')]\rangle\\
C(t,t') &=& -i\langle[\hat{B}(t,t'),\delta H(t')]\rangle\\
\delta\langle\psi'(t)|B|\psi'(t)\rangle &=& \int dt' C(t,t')
\end{eqnarray}

\section{Position operator in bloch representation}
\begin{eqnarray}\Psi(x) &=& \sum_n\int_{BZ} dk\Psi_n(k)u_{n,k}(x)e^{ik\cdot x}\\
\mbox{want }x\Psi(x) &=& \sum_n\int_{BZ} dk X\Psi_n(k)u_{n,k}(x)e^{ik\cdot x}\\
x\Psi(x) &=& x\sum_n\int_{BZ} dk\Psi_n(k)u_{n,k}(x)e^{ik\cdot x}\\
&=& \sum_n\int_{BZ} dk\Psi_n(k)u_{n,k}(x)xe^{ik\cdot x}\\
&=& \sum_n\int_{BZ} dk\Psi_n(k)u_{n,k}(x)(-i\partial_k)e^{ik\cdot x}\\
&=& \sum_n\int_{BZ} dki\partial_k(\Psi_n(k)u_{n,k}(x))e^{ik\cdot x}\\
&=& \sum_n\int_{BZ} dki\partial_k\Psi_n(k)u_{n,k}(x)+\Psi_n(k)i\partial_ku_{n,k}(x))e^{ik\cdot x}\\
&=& \sum_n\int_{BZ} dki\partial_k\Psi_n(k)u_{n,k}(x)+\Psi_n(k)\int dx'\delta(x-x')i\partial_ku_{n,k}(x'))e^{ik\cdot x}\\
&=& \sum_n\int_{BZ} dki\partial_k\Psi_n(k)u_{n,k}(x)+\Psi_n(k)\int dx'\sum_mu^\ast_{m,k}(x') u_{m,k}(x)i\partial_ku_{n,k}(x'))e^{ik\cdot x}\\
&=& \sum_n\int_{BZ} dki\partial_k\Psi_n(k)u_{n,k}(x)+\Psi_n(k)\sum_m u_{m,k}(x)\int dx'u^\ast_{m,k}(x')i\partial_ku_{n,k}(x'))e^{ik\cdot x}\\
&=& \sum_n\int_{BZ} dki\partial_k\Psi_n(k)u_{n,k}(x)+\Psi_n(k)\sum_m u_{m,k}(x)(-A_{mn}(k)))e^{ik\cdot x}\\
\end{eqnarray}

So in Bloch representation, $X = \partial_k-(A_{mn})$

\section{Orthogonality in $kq$-representation}
\begin{eqnarray}|q-q'| &<& a \mbox{ by definition} \\
|k-k'| &<& b \mbox{ by definition} \\
\psi_{kq}(x) &=& \sum_n\delta(x-q-na)e^{inka}\\
\int dx\psi_{kq}^\ast(x)\psi_{k'q'}(x) &=& \int dx\sum_{n,n'}\delta(x-q-na)e^{-inka}\delta(x-q'-n'a)e^{in'k'a}\\
&=& \int dx\sum_{n,n'}e^{in'k'a-inka}\delta(x-q-na)\delta(x-q'-n'a)\\
&=& \sum_{n,n'}e^{ia(n'k'-nk)}\delta(q-q'-(n+n')a)\\
&=& \sum_{n,n'}e^{ia(n'k'-n'k+n'k-nk)}\delta(q-q'-(n-n')a)\\
&=& \sum_{n,n'}e^{ian'(k'-k)+ia(n'-n)k)}\delta(q-q'-(n-n')a)\\
&=& \sum_{n,n'}e^{ian'(k'-k)+i(q'-q)k)}\delta(q-q'-(n-n')a)\\
&=& \sum_{n,n'}e^{ian'(k'-k))}\delta(q-q'-(n-n')a), \mbox{ because }|q-q'|<a \mbox{ and } q-q'=(n-n')a\\
\end{eqnarray}

\section{Position operator in Zak basis}
\begin{eqnarray}
\langle k'q'|p|kq\rangle &=& \int dpdp'\langle kq|p\rangle\langle p|p|p'\rangle\langle p'|l'q'\rangle \\
&=& \int dp p\langle kq|p\rangle\langle p|k'q'\rangle \\
&=& \int dp p \psi^*_{kq}(p)\psi_{k'q'}(p) \\
&=& \int dp p {1\over\sqrt a}e^{ikq}\sum_n\delta(p-k-nb)e^{iqnb} {1\over\sqrt a}e^{-ik'q'}\sum_{n'}\delta(p-k'-n'b)e^{-iq'n'b}\\
&=& \int dp p {1\over a}\sum_{n,n'}\delta(p-k-nb)\delta(p-k'-n'b)e^{ib(qn-q'n')}e^{i(kq-k'q')}\\
&=& {1\over a}\sum_{n,n'}(k+nb)\delta(k+nb-k'-n'b)e^{ib(qn-q'n')}e^{i(kq-k'q')}\\
&=& {1\over a}\sum_{n,n'}(-i){\partial\over\partial q}\delta(k+nb-k'-n'b)e^{ib(qn-q'n')}e^{i(kq-k'q')}\\
&=& -i{\partial\over\partial q}{1\over a}\sum_{n,n'}\delta(k+nb-k'-n'b)e^{ib(qn-q'n')}e^{i(kq-k'q')}\\
&=& -i{\partial\over\partial q}\delta(q-q')\delta(k-k') \mbox{ because we've already proved orthogonality} \\
\end{eqnarray}

\section{Zak combinatorial formula}
\begin{eqnarray}&& [\prod_{p=1}^mK_{i_p}][\prod_{q=1}^nK_{i_{m+q}}] \\
&=& [\prod_{p=1}^{m+n}K_p]+{1\over(m+n)!}\sum_{p=1}^m\sum_{q=1}^n[K_{i_p},K_{i_{m+q}}]\sum_{\sigma\in S_{m+n},\sigma^{-1}(p)>\sigma^{-1}(m+q)}K_{i_\sigma(1)}\ldots\hat{K}_{i_{m+q}}\hat{K}_{i_{p}}\ldots K_{i_\sigma(m+n)} \\
&=& [\prod_{p=1}^{m+n}K_p]+{(m+n)!\over(m+n-2)!}{(m+n-2)!\over(m+n)!}\sum_{p=1}^m\sum_{q=1}^n{1\over2} [K_{i_1}\ldots\hat{K}_{i_{n+q}}\ldots\hat{K}_p\ldots K_{i_{m+n}}] + \cdots \\
&=& [\prod_{p=1}^{m+n}K_p]+\sum_{\alpha=1}^3\sum_{\beta=1}^3{1\over2}[K_\alpha,K_\beta][({\partial\over\partial K_\alpha}\prod_{s=1}^m K)({\partial\over\partial K_\beta}\prod_{t=1}^n K_t)]
\end{eqnarray}

\section{Kronig-Penney}
\begin{align*}T(k, z) &=& \left(\begin{array}{ll}
e^{ikz} & 0\\
0 & e^{-ikz}\\
\end{array}
\right) & \mbox{ translate by }z\\
S(k) &=& \left(\begin{array}{ll}
1 & 1\\
ik & -ik\\
\end{array}
\right)& \mbox{convert from }\{e^{ikx},e^{-ikx}\}\mbox{ basis to }\{\psi(x), \psi'(x)\}\mbox{ basis}\\
S(k)T(k,z)S(k)^{-1} &=& \left(\begin{array}{ll}
\cos(kz) & \sin(kz)/k\\
-k\sin(kz) & \cos(kz)\\
\end{array}
\right)\\
0 &=& |S(\beta)T(\beta,b)S(\beta)^{-1}S(\alpha)T(\alpha,a)S(\alpha)^{-1}-e^{ik(a+b)}\mathbb{1}|\\
\cos((a+b)k) &=& -{\alpha^2+\beta^2\over2\alpha\beta}\sin(a\alpha)\sin(b\beta)+\cos(a\alpha)\cos(b\beta)
\end{align*}

\section{Su-Schrieffer-Heeger Model}
\begin{eqnarray}
H(\Delta) &=& t(1+\Delta)\sum_ic_{i,A}^\dagger c_{i,B}^{\hphantom{\dagger}}+t(1-\Delta)\sum_ic_{i+1,A}^\dagger c_{i,B}^{\hphantom{\dagger}}+\mbox{h.c.}+u\Delta^2 \\
\end{eqnarray}

\end{document}
